Makefile
@@ -1,7 +1,7 @@
 COQMODULE    := compcomp
 # COQTHEORIES  := $(wildcard */*.v) #*/*.v
 # COQTHEORIES  := $(shell find . -iname '*.v')
-COQTHEORIES  := $(shell find . -type d \( -path ./bound -o -path ./selfsim -o -path ./demo -o -path ./backend -o -path ./x86 -o -path ./cfrontend \) -prune -o -iname '*.v') ./backend/RenumberproofC.v ./backend/RTLC.v
+COQTHEORIES  := $(shell find . -type d \( -path ./bound -o -path ./selfsim -o -path ./demo -o -path ./backend -o -path ./x86 -o -path ./cfrontend \) -prune -o -iname '*.v') ./backend/RenumberproofC.v ./backend/RTLC.v ./backend/SeparationC.v
 
 
 .PHONY: all proof proof-quick graph
